case_study/lean/Base.lean
@@ -1,2 +1,0 @@
-import Base.Big_Step
-import Base.Small_Step
