case_study/lean/CaseStudy.lean
@@ -1,0 +1,6 @@
+import CaseStudy.Semantics.Base.Big_Step
+import CaseStudy.Semantics.Base.Small_Step
+import CaseStudy.Semantics.Hammered.Big_Step
+import CaseStudy.Semantics.Hammered.Big_Step_test
+import CaseStudy.Semantics.Hammered.Small_Step
+import CaseStudy.Semantics.Definitions.Com
