case_study/lean/CaseStudy/Semantics/Base/Big_Step.lean
@@ -1,4 +1,4 @@
-import Definitions.Com
+import CaseStudy.Semantics.Definitions.Com
 
 example (s: State) : (("x" ::= (AExp.num 5));; ("y" ::= (AExp.var "x")), s) ==> s["x" ↦ 5]["y" ↦ 5] := by
   apply BigStep.seq <;> apply BigStep.assign
@@ -21,17 +21,18 @@ theorem assign_sim (x: String) (a: AExp) (s: State) (s': State) :  (((x ::= a), 
     apply BigStep.assign
   }
 
-theorem seq_assoc : (((c1;; c2);; c3, s) ==> s') <-> ((c1;; (c2;; c3), s) ==> s') := by
-  constructor <;> 
+theorem seq_assoc {c1 c2 c3 s s'} :
+    (((c1;; c2);; c3, s) ==> s') <-> ((c1;; (c2;; c3), s) ==> s') := by
+  constructor <;>
   intro h <;>
-  cases h with 
+  cases h with
   | seq _ _ _ _ _ h1 h2
   {
-    cases h1 
+    cases h1
     repeat apply BigStep.seq <;> try assumption
   }
   {
-    cases h2 
+    cases h2
     repeat apply BigStep.seq <;> try assumption
   }
 
@@ -60,7 +61,7 @@ theorem unfold_while (c: Com) (b: BExp) : ((WHILE b DO c) ~ (IF b THEN c;; WHILE
 theorem triv_if (c: Com) (b: BExp): ((IF b THEN c ELSE c) ~ c) := by
   intros s t
   constructor
-  intro h; cases h <;> assumption 
+  intro h; cases h <;> assumption
   intro h
   cases hc: (beval b s)
   {
@@ -78,12 +79,12 @@ syntax "if_tf" : tactic
 macro_rules | `(tactic | if_tf) => `(tactic |  (first | apply BigStep.if_true; ass_triv | apply BigStep.if_false; ass_triv))
 
 syntax "ite_commute" : tactic
-macro_rules 
-  | `(tactic| ite_commute )  => `(tactic | 
+macro_rules
+  | `(tactic| ite_commute )  => `(tactic |
         first | (apply BigStep.if_true; ass_triv); if_tf | (apply BigStep.if_false; ass_triv); (try if_tf))
 
-theorem commute_if: (IF b1 THEN (IF b2 THEN c11 ELSE c12) ELSE c2) 
-   ~ 
+theorem commute_if {b1 b2 c11 c12 c2} : (IF b1 THEN (IF b2 THEN c11 ELSE c12) ELSE c2)
+   ~
    (IF b2 THEN (IF b1 THEN c11 ELSE c2) ELSE (IF b1 THEN c12 ELSE c2)) := by
   intros s t
   constructor
@@ -106,7 +107,7 @@ theorem commute_if: (IF b1 THEN (IF b2 THEN c11 ELSE c12) ELSE c2)
     }
 
 
-theorem sim_while_cong_aux:
+theorem sim_while_cong_aux {b c c' s t } :
   ((WHILE b DO c,s) ==> t)  -> (c ~ c') ->  ((WHILE b DO c',s) ==> t) := by
     intros h
     generalize rn : (WHILE b DO c, s) = p
@@ -136,7 +137,7 @@ theorem sim_while_cong_aux:
 
 
 
-theorem sim_while_cong: (c ~ c') -> (WHILE b DO c) ~ (WHILE b DO c') := by
+theorem sim_while_cong {c c' b} : (c ~ c') -> (WHILE b DO c) ~ (WHILE b DO c') := by
   intros eq s t
   constructor
   repeat (intro; apply sim_while_cong_aux; repeat assumption)
@@ -145,21 +146,21 @@ theorem sim_while_cong: (c ~ c') -> (WHILE b DO c) ~ (WHILE b DO c') := by
   symm
   assumption
 
-theorem sim_refl:  ( c ~ c ) := by
+theorem sim_refl {c} :  ( c ~ c ) := by
   intros
   trivial
 
-theorem sim_sym:   ((c ~ c') <-> (c' ~ c)) := by 
+theorem sim_sym {c c'} : ((c ~ c') <-> (c' ~ c)) := by
   constructor
   repeat (intros h s t; symm; specialize h s t; assumption)
 
-theorem sim_trans: ( (c ~ c') -> (c' ~ c'') -> (c ~ c'') ) := by 
+theorem sim_trans {c c' c''} : ((c ~ c') -> (c' ~ c'') -> (c ~ c'') ) := by
   intros h1 h2 s t
   rw [h1]
   specialize h2 s t
   assumption
 
-theorem big_step_determ: (((c,s) ==> t) ∧ ((c,s) ==> u) ) -> (u = t) := by
+theorem big_step_determ {c s t u} : (((c,s) ==> t) ∧ ((c,s) ==> u) ) -> (u = t) := by
   intro h
   rcases h with ⟨h_0, h_1⟩
   generalize rn : (c, s) = p
@@ -167,7 +168,7 @@ theorem big_step_determ: (((c,s) ==> t) ∧ ((c,s) ==> u) ) -> (u = t) := by
   induction h_0 generalizing s u c with
     | skip => cases rn; cases h_1; rfl
     | assign => cases rn; cases h_1; rfl
-    | seq _ _ _ t' _ _ _ ih ih' => 
+    | seq _ _ _ t' _ _ _ ih ih' =>
       cases rn
       cases h_1 with | seq _ _ _ v _ _ ht'
       have h_mid : (v = t') := by
@@ -185,7 +186,7 @@ theorem big_step_determ: (((c,s) ==> t) ∧ ((c,s) ==> u) ) -> (u = t) := by
       cases h_1 with
         | if_true => trivial
         | if_false => apply ih; assumption; rfl
-    | while_true _ _ _ t' _ _ _ _ ih ih' => 
+    | while_true _ _ _ t' _ _ _ _ ih ih' =>
       cases rn
       cases h_1 with
         | while_true _ _ _ v _ _ hbody _ =>
