case_study/lean/Hammered.lean
@@ -1,3 +1,0 @@
-import Hammered.Big_Step
-import Hammered.Big_Step_test
-import Hammered.Small_Step
