case_study/lean/Main.lean
@@ -1,6 +1,0 @@
-import Definitions
-import Base
-import Hammered
-
-def main : IO Unit :=
-  IO.println s!"Hello, world!"
